src/AtomicPair/AtomicPairAPI.v
@@ -27,10 +27,12 @@ Module Type AtomicPairAPI.
 
   Parameter abstr : Abstraction State.
 
+  Axiom init_ok : init_abstraction init recover abstr inited_any.
   Axiom get_ok : prog_spec get_spec get recover abstr.
   Axiom put_ok : forall v, prog_spec (put_spec v) (put v) recover abstr.
   Axiom recover_noop : rec_noop recover abstr no_wipe.
 
+  Hint Resolve init_ok.
   Hint Resolve get_ok.
   Hint Resolve put_ok.
   Hint Resolve recover_noop.
