src/BadSectorDisk/BadSectorAPI.v
@@ -53,12 +53,14 @@ Module Type BadSectorAPI.
 
   Axiom abstr : Abstraction State.
 
+  Axiom init_ok : init_abstraction init recover abstr inited_any.
   Axiom read_ok : forall a, prog_spec (read_spec a) (read a) recover abstr.
   Axiom write_ok : forall a v, prog_spec (write_spec a v) (write a v) recover abstr.
   Axiom getBadSector_ok : prog_spec getBadSector_spec getBadSector recover abstr.
   Axiom diskSize_ok : prog_spec diskSize_spec diskSize recover abstr.
   Axiom recover_noop : rec_noop recover abstr no_wipe.
 
+  Hint Resolve init_ok.
   Hint Resolve read_ok.
   Hint Resolve write_ok.
   Hint Resolve getBadSector_ok.
