src/BadSectorDisk/BadSectorImpl.v
@@ -15,6 +15,7 @@ Module BadSectorDisk <: BadSectorAPI.
 
   Axiom abstr : Abstraction State.
 
+  Axiom init_ok : init_abstraction init recover abstr inited_any.
   Axiom read_ok : forall a, prog_spec (read_spec a) (read a) recover abstr.
   Axiom write_ok : forall a v, prog_spec (write_spec a v) (write a v) recover abstr.
   Axiom getBadSector_ok : prog_spec getBadSector_spec getBadSector recover abstr.
